\textbf{Solução} Note que
\begin{equation}
S_n^2 = (n-1)^{-1} \sum_{i=2}^n Y_i^2 \quad \text{para} \quad Y_i \sim N(0, \sigma^2),
\end{equation}
em que $Y_1, \ldots, Y_n$ são v.a.'s de Helmert.

Além disso,
\begin{equation}
\mathrm{Var}(Y_i^2) = \mathbb{E}[Y_i^4] - \mathbb{E}^2[Y_i^2]
\end{equation}
\begin{equation}
= 3\sigma^4 - \sigma^4 = 2\sigma^4 < \infty, \quad \text{uma vez que:}
\end{equation}

Como
\begin{equation}
M_{Y_i^2}(t) = e^{\frac{t^2\sigma^2}{2}}
\end{equation}

\begin{equation}
\left. \frac{d M_{Y_i^2}(t)}{dt} \right|_{t=0} = \left. \frac{d}{dt} e^{\frac{t^2\sigma^2}{2}} \right|_{t=0} = t\sigma^2 e^{\frac{t^2\sigma^2}{2}} \bigg|_{t=0} = 0 = \mathbb{E}(Y_i)
\end{equation}

\begin{equation}
\left. \frac{d^2 M_{Y_i^2}(t)}{dt^2} \right|_{t=0} = t^2\sigma^4 e^{\frac{t^2\sigma^2}{2}} + \sigma^2 e^{\frac{t^2\sigma^2}{2}} \bigg|_{t=0} = \sigma^2 = \mathbb{E}(Y_i^2)
\end{equation}

\begin{equation}
\left. \frac{d^3 M_{Y_i^2}(t)}{dt^3} \right|_{t=0} = t^3\sigma^6 e^{\frac{t^2\sigma^2}{2}} + 2t\sigma^4 e^{\frac{t^2\sigma^2}{2}} + t\sigma^4 e^{\frac{t^2\sigma^2}{2}} \bigg|_{t=0} = 0 = \mathbb{E}(Y_i^3)
\end{equation}

\begin{equation}
\begin{aligned}
\left. \frac{d^4 M_{Y_i^2}(t)}{dt^4} \right|_{t=0} &= t^4\sigma^8 e^{\frac{t^2\sigma^2}{2}} + 3t^2\sigma^6 e^{\frac{t^2\sigma^2}{2}} \\
&\quad + 2t^2\sigma^6 e^{\frac{t^2\sigma^2}{2}} + 2\sigma^4 e^{\frac{t^2\sigma^2}{2}} + t^2\sigma^6 e^{\frac{t^2\sigma^2}{2}} + \sigma^4 e^{\frac{t^2\sigma^2}{2}} \bigg|_{t=0} \\
&= 3\sigma^4 = \mathbb{E}(Y_i^4)
\end{aligned}
\end{equation}