\[
= 1 - F_{T_n}(\theta (1 - \frac{u}{n}))
\]
\[
= 1 - \left(1 - \frac{u}{n}\right)^n, \quad u > 0.
\]

Daí,
\[
\lim_{n \to \infty} F_{U_n}(u) = 1 - e^{-u} = F_U(u), \quad \text{que é a fda de } E \in \text{EXP}(1).
\]
Então,
\[
U_n \xrightarrow[n \to \infty]{} E.
\]

\textbf{Resultado 1D:} Sejam $\{U_n, n \geq 1\}$ uma sequência de v.a.'s tal que $M_{U_n}(t)$ é a fgm de $U_n$ e $U$ uma v.a. com fgm $M_U(t)$, então
\[
\text{Se } M_{U_n}(t) \xrightarrow[n \to \infty]{} M_U(t), \text{ então } U_n \xrightarrow[n \to \infty]{} U.
\]

\textbf{Q (extra 6)} Sejam $X_1, \ldots, X_n$ v.a.'s i.i.d. tais que $X_i \sim \text{Bernoulli}(p)$ com $p = \frac{1}{2}$ e 
\[
U_n = 2 \sqrt{n} \left( \bar{X}_n - \frac{1}{2} \right).
\]
Estude a distribuição limite de $U_n$.

\textbf{Solução:} Note que 
\[
U_n = \frac{2 \sum_{i=1}^n X_i - n}{\sqrt{n}}.
\]
\[
M_{U_n}(t) = E\left[ e^{\frac{2t}{\sqrt{n}} \sum_{i=1}^n X_i - t \sqrt{n}} \right] 
= e^{-t \sqrt{n}} E\left[ e^{\frac{2t}{\sqrt{n}} \sum_{i=1}^n X_i} \right]
\]
\[
= e^{-t \sqrt{n}} \left( E\left[ e^{\frac{2t}{\sqrt{n}} X_1} \right] \right)^n
\]
\[
= e^{-t \sqrt{n}} \left( (1-p) + p \cdot e^{\frac{2t}{\sqrt{n}}} \right)^n
\]