\textbf{Prova:} \\
Considere
\begin{equation}
\sqrt{n} \left[ g(T_n) - g(\theta) \right] = U_n \cdot V_n,
\end{equation}
em que
\begin{equation}
U_n = \sqrt{n} (T_n - \theta) \quad \text{e} \quad V_n = \frac{g(T_n) - g(\theta)}{T_n - \theta}.
\end{equation}

Note que 
\begin{equation}
T_n - \theta = \frac{U_n}{\sqrt{n}}.
\end{equation}

Como
\begin{equation}
U_n \xrightarrow{d} N(0, \sigma^2) \quad \text{e} \quad \frac{1}{\sqrt{n}} \xrightarrow{P}_{n \to \infty} 0, \quad \text{do Teo. Slutsky},
\end{equation}
temos
\begin{equation}
T_n - \theta \xrightarrow{P}_{n \to \infty} 0.
\end{equation}

Daí, 
\begin{equation}
V_n \xrightarrow{P}_{n \to \infty} g'(\theta), \quad \text{pela definição}
\end{equation}
\begin{equation}
g'(x) = \lim_{g \to x} \frac{g(x) - g(z)}{g - x}.
\end{equation}

Assim, pelo Teo. Slutsky,
\begin{equation}
\sqrt{n} \left[ g(T_n) - g(\theta) \right] \xrightarrow{d}_{n \to \infty} N\left(0, \left[ g'(\theta) \right]^2 \sigma^2 \right).
\end{equation}

\textbf{Q (extra 10)} \\
Sejam $X_1, \ldots, X_n$ v.a.'s i.i.d. tais que $X_i \sim \text{Poisson}(\lambda)$. Encontre a distribuição assintótica de 
\begin{equation}
\sqrt{n} \left( \overline{X_n^3} - \lambda^3 \right).
\end{equation}

\textbf{Solução} \\
Pode-se mostrar que
\begin{equation}
E\{ X_i^3 \} = \lambda < \infty \quad \text{e} \quad \text{Var}\{ X_i^3 \} = \lambda < \infty.
\end{equation}
Pelo Teo. (3.7.6.1(a)).