\section*{Teorema (3.7.6.3(a)) [TCL para variância amostral]}

Sejam $X_1, \dots, X_n$ v.a.'s i.i.d. com média $\mu$, variância $\sigma^2$ e $\mu_4 = \mathbb{E}[(X_1 - \mu)^4]$. Assuma que $0 < \mu_4 < \infty$ e $\mu_4 > \sigma^4$ (curtose $> 1$). Então,
\begin{equation}
\sqrt{n} \left( S_n^2 - \sigma^2 \right) \xrightarrow[n \to \infty]{d} N\left(0, \mu_4 - \sigma^4\right)
\end{equation}

\subsection*{Prova:}

Considere 
\[
W_n \triangleq (n-1) n^{-1} S_n^2, \quad Y_i \triangleq (X_i - \mu)^2 \quad \text{para } i = 1, \dots, n
\]
e 
\[
\overline{Y}_n = n^{-1} \sum_{i=1}^n Y_i.
\]

Assim,
\begin{align}
W_n &= \frac{1}{n} \sum_{i=1}^n (X_i - \overline{X}_n)^2 \\
&= \frac{1}{n} \sum_{i=1}^n \left( X_i - \mu + \mu - \overline{X}_n \right)^2 \\
&= \frac{1}{n} \sum_{i=1}^n \left[ (X_i - \mu)^2 + 2(X_i - \mu)(\mu - \overline{X}_n) + (\mu - \overline{X}_n)^2 \right] \\
&= \frac{1}{n} \sum_{i=1}^n (X_i - \mu)^2 - 2(\overline{X}_n - \mu)^2 + (\overline{X}_n - \mu)^2 \\
&= \overline{Y}_n - (\overline{X}_n - \mu)^2
\end{align}

Ainda, vale-se
\begin{align}
\sqrt{n} \left( W_n - \sigma^2 \right) &= \sqrt{n} \left( \overline{Y}_n - \sigma^2 \right) - \sqrt{n} \left( \overline{X}_n - \mu \right)^2 \\
&= U_n + V_n
\end{align}

Note que $\{ Y_i \} \stackrel{\text{i.i.d.}}{\sim} \left[ \mathbb{E}[Y_i] = \sigma^2, \ \mathrm{Var}(Y_i) = \mu_4 - \sigma^4 \right]$.