\textbf{Ex:} $n^2 = O(6n^2 + n)$ pois
\begin{equation}
\frac{n^2}{6n^2 + n} = \frac{1}{6 + n^{-1}} \leq \frac{1}{6}, \quad \forall n \geq 1
\end{equation}

\[
\frac{n^2}{6n^2 + n} = \frac{1}{6 + n^{-1}} \leq \frac{1}{6 + (1)^{-1}} = \frac{1}{7}
\]

$a_n = \theta(b_n)$ se, sse, $\forall \varepsilon > 0, \exists n_0 = n_0(\varepsilon): \frac{a_n}{b_n} \leq \varepsilon, \ \forall n \geq n_0$, isto é, $\lim_{n \to \infty} \frac{a_n}{b_n} = 0$. Em particular, $a_n = \theta(1)$ implica que
\begin{equation}
\lim_{n \to \infty} a_n = 0
\end{equation}

\textbf{Ex:} $n = \theta(n^2)$ pois
\begin{equation}
\frac{n}{n^2} = \frac{1}{n} \xrightarrow[n \to \infty]{} 0
\end{equation}

\textbf{Ex:} $n^{-1} = \theta(1)$ pois
\begin{equation}
\frac{1}{n} \xrightarrow[n \to \infty]{} 0
\end{equation}

\textbf{Teorema (Extra 1) [Propriedades de $O(\cdot)$ e $\theta(\cdot)$]} \\
Sejam $\{a_n, n \geq 1\}$, $\{b_n, n \geq 1\}$, $\{c_n, n \geq 1\}$ e $\{d_n, n \geq 1\}$ sequências de números reais, valem-se:

\begin{itemize}
    \item[(i)] Se $a_n = O(b_n)$, então $a_n = o(b_n)$.
    \item[(ii)] Se $a_n = O(b_n)$ e $c_n = O(d_n)$, então ...
\end{itemize}